rupicola/stlc_v2/SyntacticTypes.fst
@@ -118,3 +118,9 @@ let lem_gsubst_empty_identity (e:closed_exp) :
   Lemma (gsubst gsub_empty e == e)
   [SMTPat (gsubst gsub_empty e)] =
   admit ()
+**)
+
+let lem_gsubst_closed_identiy #g #b (s:gsub g b) (e:closed_exp) :
+  Lemma (gsubst s e == e)
+  [SMTPat (gsubst s e)] =
+  admit ()
